theories/Interp.v
@@ -1,4 +1,7 @@
 (* begin hide *)
+From Coinduction Require Import
+     coinduction rel tactics.
+
 From ExtLib Require Import
      Structures.Functor
      Structures.Monad.
@@ -7,7 +10,7 @@ From ITree Require Import
 	Basics.Basics.
 
 From CTree Require Import
-		 Utils CTrees Equ Bisim.
+		 Utils CTrees Equ Bisim CTreesTheory.
 
 Import CTreeNotations.
 Open Scope ctree_scope.
@@ -38,39 +41,33 @@ Definition interp {E M : Type -> Type}
 			iter (fun t =>
 				match observe t with
 				| RetF r => ret (inr r)
-				| @ChoiceF _ _ _ _ n k => bind (choice n) (fun x => ret (inl (k x)))
+				| @ChoiceF _ _ _ b n k => bind (choice b n) (fun x => ret (inl (k x)))
 				| VisF e k => fmap (fun x => inl (k x)) (h _ e)
 				end).
 
 Arguments interp {E M FM MM IM FoM} h [T].
 
-(*
 (** Unfolding of [interp]. *)
 Notation interp_ h t :=
-         (* {E F R} (h : E ~> ctree F) (ot : ctreeF E R _) : ctree F R := *)
   (match observe t with
   | RetF r => Ret r
-	| VisF e k => fmap (fun x => TauI (interp h (k x))) (h _ e)
-	| @ChoiceF _ _ _ _ n k => bind (choice n) (fun x => ret (inl (k x)))
-  end).
-
+	| VisF e k => bind (h _ e) (fun x => TauI (interp h (k x)))
+	| @ChoiceF _ _ _ b n k => bind (choice b n) (fun x => TauI (interp h (k x)))
+  end)%function.
 
 (** Unfold lemma. *)
-Lemma unfold_interp {E F R} {h : E ~> ctree F} (t : ctree E R) : 
-  interp h t ≅ match observe t with
-          | RetF r => Ret r
-          | VisF e k => x <- h _ e;; TauI (interp h (k x))
-          | ChoiceF b n k => Choice b n (fun i => (interp h (k i)))
-          end.
+Lemma unfold_interp {E F R} {h : E ~> ctree F} (t : ctree E R) :
+  interp h t ≅ interp_ h t.
 Proof.
   unfold interp, Basics.iter, MonadIter_ctree.
   rewrite unfold_iter.
   destruct (observe t); cbn.
-  - now rewrite ?bind_ret_l. 
-  - now rewrite ?bind_ret_l. 
+  - now rewrite ?bind_ret_l.
+  - now rewrite bind_map, ?bind_ret_l.
+  - rewrite bind_bind.
+    setoid_rewrite bind_ret_l.
+    reflexivity.
 Qed.
-
-
 
 (** ** [interp] and constructors *)
 
@@ -78,18 +75,27 @@ Qed.
     rewrite hints.
  *)
 
-Lemma interp_ret {E F R} {f : E ~> itree F} (x: R):
+Lemma interp_ret {E F R} {f : E ~> ctree F} (x: R):
   interp f (Ret x) ≅ Ret x.
-Proof. rewrite unfold_interp. reflexivity. Qed.
+Proof. now rewrite unfold_interp. Qed.
 
-Lemma interp_tau {E F R} {f : E ~> itree F} (t: itree E R):
-  eq_itree eq (interp f (Tau t)) (Tau (interp f t)).
-Proof. rewrite unfold_interp. reflexivity. Qed.
+Lemma interp_tau {E F R} {f : E ~> ctree F} (t: ctree E R):
+  interp f (TauI t) ≅ TauI (TauI (interp f t)).
+Proof.
+  rewrite unfold_interp.
+  cbn.
+  unfold choice, MonadChoice_ctree, CTree.choice. cbn.
+  rewrite unfold_bind.
+  cbn.
+  setoid_rewrite bind_ret_l.
+  reflexivity.
+Qed.
 
-Lemma interp_vis {E F R} {f : E ~> itree F} U (e: E U) (k: U -> itree E R) :
-  eq_itree eq (interp f (Vis e k)) (ITree.bind (f _ e) (fun x => Tau (interp f (k x)))).
-Proof. rewrite unfold_interp. reflexivity. Qed.
+Lemma interp_vis {E F R} {f : E ~> ctree F} U (e: E U) (k: U -> ctree E R) :
+  interp f (Vis e k) ≅ x <- f _ e;; TauI (interp f (k x)).
+Proof. now rewrite unfold_interp. Qed.
 
+(*
 Lemma interp_trigger {E F : Type -> Type} {R : Type}
       (f : E ~> (itree F))
       (e : E R) :
